Term.fvs_subst

DeBruijnSSA/BinSyntax/Syntax/Fv/Subst.lean
@@ -31,6 +31,24 @@ theorem BBRegion.fl_vsubst (σ : Term.Subst φ) (r : BBRegion φ) : (r.vsubst σ
 theorem Region.fl_vsubst (σ : Term.Subst φ) (r : Region φ) : (r.vsubst σ).fl = r.fl := by
   induction r generalizing σ <;> simp [*]
 
+def Term.Subst.fvs (σ : Term.Subst φ) (i : ℕ) : Set ℕ := (σ i).fvs
+
+theorem Term.fvs_subst (σ : Term.Subst φ) (t : Term φ) : (t.subst σ).fvs = ⋃ x ∈ t.fvs, σ.fvs x
+  := by induction t with
+  | pair a b Ia Ib =>
+    ext k
+    simp only [fvs, Ia, Subst.fvs, Ib, Set.mem_union, Set.mem_iUnion, exists_prop]
+    constructor
+    intro h
+    cases h with
+    | inl h => exact have ⟨x, h, hk⟩ := h; ⟨x, Or.inl h, hk⟩
+    | inr h => exact have ⟨x, h, hk⟩ := h; ⟨x, Or.inr h, hk⟩
+    intro ⟨x, h, hk⟩
+    cases h with
+    | inl h => exact Or.inl ⟨x, h, hk⟩
+    | inr h => exact Or.inr ⟨x, h, hk⟩
+  | _ => simp [Subst.fvs, *]
+
 -- TODO: Term.Subst.fv
 
 -- TODO: {Terminator, Region}.Subst.{fv, fl}
